theories/tree_test.v
@@ -29,13 +29,15 @@ Notation app x y := (Tm_App x y).
 
 Coercion Tm_P : P >-> Tm.
 
-Definition s1 : Sigma := [fmap].[fresh [fset IV 0] <- Tm_P tt].
-Definition s2 : Sigma := [fmap].[fresh [fset IV 0] <- Tm_P ff].
+Definition s1 : Sigma := [fmap].[IV 1 <- Tm_P tt].
+Definition s2 : Sigma := [fmap].[IV 1 <- Tm_P ff].
 
 Lemma vars_sigma_set v s: vars_sigma fmap0.[v <- s] = v |` vars_tm s.
 Proof. by rewrite /vars_sigma/= /codom_vars codom0_set/= !fsetU0. Qed.
 
-Definition simpl_set:= (fsetU0, fset0U, codomf0, cat0f, vars_sigma0, fsetUid, acyclic_sigma0, deref_P, ren_P, ren_app, deref_empty, vars_sigma_set, unify_refl, cardfs1).
+Definition simpl_set:= (fsetU0, fset0U, codomf0, cat0f, vars_sigma0, fsetUid, acyclic_sigma0, deref_P, ren_P, ren_app, deref_empty, vars_sigma_set, unify_refl, cardfs1, freshUU, freshP0, freshP1).
+
+Ltac sif := simpl (if _ then _ else _); cbn match.
 
 Section Test1.
 
@@ -46,52 +48,92 @@ Section Test1.
       mkR (app q tt) [:: call (app p v0) ; call (app r v0) ] 
     ].
 
-  Goal exists v, runT unif p_test fset0 fmap0 (Unexplored (call (app q tt))) (One s2) false v.
+(*   Lemma varsU_set (m: Sigma) k t:
+    k \notin domf m ->
+    codom m.[k <- t] = t :: codom m.
+  Proof.
+    move=> H.
+    rewrite codomE [domf _]/=.
+    rewrite/=.
+    Search (enum (_ `|` _)).
+    Search enum 
+    Search (domf (_ `|` _)).
+    
+    Search codom (_.[_ <- _]).
+    rewrite/=. *)
+
+  Goal exists v, runT unif p_test 0 fmap0 (Unexplored (call (app q tt))) (One s2) false v.
   Proof.
     repeat eexists.
-    set X := [fset IV 0; fresh [fset IV 0]].
+    have PV : v_prog (rules p_test) = [fset IV 0].
+      by rewrite/v_prog/=/varsU_rule/varsU_rhead/varsU_rprem/vars_atoms/=!simpl_set.
+
     apply: StepT' => //=; cycle 1.
-      rewrite/bc.
-      rewrite deref_App [vars_tm _]/= !simpl_set.
-      rewrite/= !simpl_set.
-      rewrite/fresh_rule /varsU_rule/varsU_rhead/varsU_rprem/=.
-      rewrite !simpl_set FmapE.fmapE/= !inE/=.
-      rewrite/rename/= !inE/= !FmapE.fmapE/=.
-      rewrite in_fnd?inE//= => H.
-      by rewrite ffunE unify_refl/= !simpl_set//.
-    set Z := (_ `|` _).
-    set K := (fresh _).
+      rewrite/bc; rewrite PV.
+      rewrite vars_sigma0 !simpl_set /maxn; sif.
+      rewrite/fresh_rule/= !FmapE.fmapE !inE eqxx orbF.
+      rewrite !FmapE.fmapE eqxx [odflt _ _]/=.
+      set X := select _ _ _ _ _.
+      have : [:: ([fmap], [:: call (app p (Tm_V (IV 1))); call (app r (Tm_V (IV 1)))])]  = X.
+        rewrite/X select_cons/get_input_vars !FmapE.fmapE eqxx.
+        do 2 case: eqP => // _.
+        rewrite/build_arr/H [head _]/=.
+        cbn match.
+        case: eqP => // _.
+        rewrite select_cons/get_input_vars !FmapE.fmapE eqxx.
+        do 2 case: eqP => // _.
+        rewrite simpl_set/build_arr/H [head _]/=.
+        cbn match.
+        case: eqP => // _.
+        rewrite select_cons/get_input_vars !FmapE.fmapE eqxx.
+        do 2 case: eqP => // _.
+        rewrite/build_arr/H [head _]/=.
+        cbn match.
+        case: eqP => // _.
+        rewrite select_cons/get_input_vars !FmapE.fmapE eqxx.
+        rewrite/build_arr/H [head _]/=.
+        cbn match.
+        case: eqP => // _.
+        rewrite !FmapE.fmapE eqxx.
+        do 2 case: eqP => // _.
+        rewrite [omap _ _]/=; cbn match.
+        rewrite fsetU0  ![omap _ _]/= unify_refl [omap _ _]/=.
+        rewrite//=.
+      move=><-.
+      rewrite/=/vars_atoms/= !freshUU !freshP1 codom_vars0 freshP0/=.
+      rewrite/maxn//=.
+
     apply: StepT => //=.
-      rewrite/bc deref_App !simpl_set.
-      rewrite [fresh_rules _ _]/= /fresh_rule !simpl_set.
-      rewrite/rename [fresh_tm _ _ _]/= !simpl_set.
-      rewrite /= !simpl_set /rename/= !simpl_set !inE /=.
-      rewrite !FmapE.fmapE/=.
-      by rewrite !unify_V_0r.
-    set R := (_ `|` _).
+      rewrite/bc vars_sigma0 PV !simpl_set /maxn; sif.
+      rewrite /fresh_rule/= !FmapE.fmapE !inE eqxx orbF.
+      set X := select _ _ _ _ _.
+      have : X = [:: ([fmap].[IV 1 <- Tm_P tt], [::]); ([fmap].[IV 1 <- Tm_P ff], [::])] .
+        rewrite/X/= !FmapE.fmapE.
+        do 4 case: eqP => // _.
+        rewrite/build_arr/=.
+        rewrite unify_V_0r//.
+        by rewrite/=unify_V_0r//=.
+      move=> ->{X}/=.
+      rewrite/vars_sigma/codom_vars/vars_atoms freshP0 !codom0_set/= !simpl_set.
+      by rewrite/maxn/=.
     apply: StepT => //.
-      rewrite/step/=.
-      rewrite/bc /next_subst [next _ _]/= acyclic_sigma_set_D//.
-      rewrite deref_App deref_P /get_tm_hd.
-      rewrite/= !simpl_set.
-      rewrite /fresh_rule/= !simpl_set.
-      rewrite/rename [fresh_tm _ _ _]/= !simpl_set.
-      rewrite !inE/= !simpl_set !FmapE.fmapE/=.
-      rewrite in_fnd/=?inE// => JK.
-      rewrite ffunE/= eqxx.
-      rewrite unify_ground//=.
-    rewrite !simpl_set fsetUC.
-    set T := (_ `|` _).
+      rewrite/=/bc/next_subst [next _ _]/= acyclic_sigma_set_D//.
+      rewrite deref_App PV deref_V FmapE.fmapE eqxx [vars _]/=.
+      rewrite vars_sigma_set !simpl_set /maxn; sif.
+      rewrite /fresh_rule/= !inE eqxx !FmapE.fmapE eqxx orbF.
+      set X := select _ _ _ _ _.
+      have : X = [::] by rewrite/X/= !simpl_set !FmapE.fmapE/=unify_ground.
+      by move=> ->{X}/=.
     apply: BackT => //=.
-    apply: StepT => //=.
-      rewrite /bc.
-      rewrite/next_subst/= acyclic_sigma_set_D//=.
-      rewrite !FmapE.fmapE/= !simpl_set.
-      rewrite/= /fresh_rule/= !simpl_set.
-      rewrite /rename/= !simpl_set in_fset1/=.
-      rewrite !FmapE.fmapE/= not_fnd//=.
-      rewrite eqxx/= unify_ground//.
-    rewrite !simpl_set/=.
+    apply: StepT => //.
+      rewrite/=/bc/next_subst [next _ _]/= acyclic_sigma_set_D//.
+      rewrite deref_App PV deref_V FmapE.fmapE eqxx [vars _]/=.
+      rewrite vars_sigma_set !simpl_set /maxn; sif.
+      rewrite /fresh_rule/= !inE eqxx !FmapE.fmapE eqxx orbF.
+      set X := select _ _ _ _ _.
+      have : X = [:: ([fmap].[IV 1 <- Tm_P ff], [::])].
+        by rewrite/X/=!FmapE.fmapE eqxx/= unify_refl/=.
+      move=>->{X}/=; rewrite/maxn !simpl_set//=.
     apply: StopOT => //=.
     by [].
   Qed.
@@ -105,21 +147,21 @@ Section Test5.
       mkR (app q ff) [::] 
     ].
 
-  Goal exists v, runT unif p_test1 fset0 fmap0 (Unexplored (call (app p ff))) (One s1) false v.
+  Goal exists v, runT unif p_test1 0 fmap0 (Unexplored (call (app p ff))) (One s1) false v.
   Proof.
     repeat eexists.
     apply: StepT' => //=; cycle 1.
       rewrite/bc.
-      rewrite !simpl_set.
-      rewrite[fresh_rules _ _]/= !simpl_set/= !FmapE.fmapE/=.
-      rewrite !inE/=.
-      by rewrite /varsU_rule/varsU_rhead/varsU_rprem/=/vars_atoms/= !simpl_set/=.
-    set X := _ `|` _.
+      rewrite !simpl_set !maxnn.
+      rewrite[fresh_rules _ _]/= !simpl_set/= !FmapE.fmapE/=simpl_set [omap _ _]/=; sif.
+      rewrite in_fnd?inE//= => H.
+      rewrite ffunE [val _]/={H} eqxx/vars_atoms/= !simpl_set/maxn//=.
     apply: StepT => //=.
-      rewrite/bc/=.
-      rewrite !FmapE.fmapE/= in_fnd//=?inE//= => H.
-      rewrite ffunE/= not_fnd//= unify_V_0r//=.
-      rewrite unify_V_0r//= acyclic_sigma0//=.
+      rewrite/bc.
+      rewrite !simpl_set !maxnn.
+      rewrite[fresh_rules _ _]/= !simpl_set/= !FmapE.fmapE/= [omap _ _]/=; sif.
+      rewrite !unify_V_0r/=/vars_atoms/=; only 2-5: by [].
+      by rewrite freshP0 vars_sigma_set !simpl_set /maxn//=.
     apply/StepT => //=.
     apply/StopOT => //=.
     by [].
@@ -135,25 +177,27 @@ Section Test6.
       mkR (app q ff) [::] 
   ].
 
-  Goal exists r, runT unif p_test2 fset0 fmap0 (Unexplored (call (app p tt)) ) (One s1) false r.
+  Goal exists r, runT unif p_test2 0 fmap0 (Unexplored (call (app p tt)) ) (One s1) false r.
   Proof.
     repeat eexists.
     apply: StepT' => //; cycle 1.
-      rewrite/=/bc/=.
-      rewrite !FmapE.fmapE not_fnd//= !simpl_set/=.
-      rewrite in_fnd//=?inE// => H; rewrite !inE/= ffunE//=.
-    set X:= (_ `|` _).
+      rewrite/=/bc.
+      rewrite !simpl_set !maxnn.
+      rewrite[fresh_rules _ _]/= !simpl_set/= !FmapE.fmapE/=simpl_set [omap _ _]/=; sif.
+      rewrite in_fnd?inE//= => H.
+      rewrite ffunE [val _]/={H} eqxx/vars_atoms/= !simpl_set/maxn//=.
     apply: StepT => //=.
-      rewrite/bc/=.
-      by rewrite acyclic_sigma0/= !FmapE.fmapE/= not_fnd//= !unify_V_0r//=.
-    rewrite /varsU_rule/varsU_rhead/varsU_rprem/=/vars_atoms/= !simpl_set/=.
-    set Y := _ `|` _.
+      rewrite/bc.
+      rewrite !simpl_set !maxnn.
+      rewrite[fresh_rules _ _]/= !simpl_set/= !FmapE.fmapE/= !unify_V_0r; only 2-5: by [].
+      
+      by rewrite/=/vars_atoms !simpl_set/maxn//=.
     apply/StepT => //=.
-      rewrite/next_subst/=.
-      rewrite/bc /=!simpl_set/=.
-      rewrite acyclic_sigma_set_D//=.
-      by rewrite !FmapE.fmapE.
-    rewrite !simpl_set.
+      rewrite/next_subst[next _ _]/=.
+      rewrite/=/bc.
+      rewrite !simpl_set !maxnn.
+      rewrite[fresh_rules _ _]/= !simpl_set/= !FmapE.fmapE/= simpl_set acyclic_sigma_set_D ?[negb _]/=; last by [].
+      by sif; rewrite !simpl_set /maxn//=.
     apply: StepT => //=.
     apply: StopOT => //=.
     by [].
@@ -165,40 +209,40 @@ Definition emptyp := (build_progr [::]).
 Definition CutS := Unexplored cut.
 
 Section Test2.
-  Goal step unif emptyp fset0 fmap0 (Or (Some OK) fmap0 OK) = (fset0, Success, Or (Some OK) fmap0 OK). by []. Qed.
+  Goal step unif emptyp 0 fmap0 (Or (Some OK) fmap0 OK) = (0, Success, Or (Some OK) fmap0 OK). by []. Qed.
 
-  Goal runT unif emptyp fset0 fmap0 (Or (Some CutS) fmap0 OK) (One fmap0) false fset0.
+  Goal runT unif emptyp 0 fmap0 (Or (Some CutS) fmap0 OK) (One fmap0) false 0.
     apply: StepT' => //=; cycle 1.
     apply: StopOT => //.
     by [].
   Qed.
 
   Goal forall r, 
-    runT unif emptyp fset0 fmap0 (Or (Some CutS) fmap0 r) (One fmap0) false fset0.
+    runT unif emptyp 0 fmap0 (Or (Some CutS) fmap0 r) (One fmap0) false 0.
     move=> r.
     apply: StepT' => //; cycle 1.
     apply: StopOT => //=.
     by [].
   Qed.
 
-  Goal runT unif emptyp fset0 fmap0 (Or (Some OK) fmap0 (Or (Some OK) fmap0 OK)) (Many fmap0 (Or None fmap0 (Or (Some OK) fmap0 OK))) false fset0.
+  Goal runT unif emptyp 0 fmap0 (Or (Some OK) fmap0 (Or (Some OK) fmap0 OK)) (Many fmap0 (Or None fmap0 (Or (Some OK) fmap0 OK))) false 0.
   Proof. apply: StopMT => //=. Qed.
 
   (* (Dead \/ !) \/ C *)
-  Goal step unif emptyp fset0 fmap0 (Or (Some (Or None fmap0 (CutS))) fmap0 OK) = (fset0, Expanded, (Or (Some (Or None fmap0 OK)) fmap0 OK)).
+  Goal step unif emptyp 0 fmap0 (Or (Some (Or None fmap0 (CutS))) fmap0 OK) = (0, Expanded, (Or (Some (Or None fmap0 OK)) fmap0 OK)).
   Proof.
     move=>//=.
   Qed.
 End Test2.
 
 Section map.
-  Definition cons := IP 501.
-  Definition nil := IP 502.
-  Definition one := IP 503.
-  Definition two := IP 504.
-  Definition four := IP 505.
-  Definition map := IP 600.
-  Definition double := IP 601.
+  Definition cons := IP 1.
+  Definition nil := IP 2.
+  Definition one := IP 3.
+  Definition two := IP 4.
+  Definition four := IP 5.
+  Definition map := IP 6.
+  Definition double := IP 7.
 
   Definition mapS := arr input (arr input exp (arr output exp func)) (arr input exp (arr output exp func)).
   Definition consS := arr output exp exp.
@@ -206,17 +250,17 @@ Section map.
   Definition oneS := exp.
   Definition twoS := exp.
   Definition fourS := exp.
-  Definition doubleS := arr input exp func.
+  Definition doubleS := arr input exp (arr output exp func).
 
-  Definition X := IV 300.
-  Definition X' := IV 301.
-  Definition Y := IV 400.
-  Definition Y' := IV 401.
-  Definition F := IV 500.
+  Definition X := IV 8.
+  Definition X' := IV 9.
+  Definition Y := IV 10.
+  Definition Y' := IV 11.
+  Definition F := IV 12.
 
   Coercion Tm_V : V >-> Tm.
-
-  Definition p' := {|
+  
+  Definition mk_p F X Y X' Y' := {|
     sig := [fmap].[map <- mapS].[double <- doubleS];
     rules := 
       mkR (app (app (app map F) nil) nil) [::] ::
@@ -225,18 +269,14 @@ Section map.
       mkR (app (app double one) two) [::]
       :: [::]
   |}.
+    
+
+  Definition p' := mk_p F X Y X' Y'.
 
   Definition list12 := app (app cons one) nil.
   Definition list24 := app (app cons two) nil.
 
   Definition map12d := app (app (app map double) list12) X.
-
-  (* Lemma get_input_vars_ground m T:
-    all ground T -> get_input_vars m T = fset0.
-  Proof.
-    elim: m T => //[x xs IH] []//= X XS /andP[G1 G2].
-    by rewrite IH// ground_vars_tm// fset0U if_same.
-  Qed. *)
 
   Lemma p'map: (sig p').[? map] = Some mapS.
   Proof. by rewrite !FmapE.fmapE. Qed.
@@ -250,20 +290,7 @@ Section map.
   Lemma fstS T1 T2 (a:T1) (b:T2): (a,b).1 = a. by []. Qed.
   Lemma sndS T1 T2 (a:T1) (b:T2): (a,b).2 = b. by []. Qed.
 
-  (* Lemma select_cons m ft md x xs s: select u m ft md (x::xs) s = 
-    (if inl m != get_tm_hd (head x)
-      then select u m ft md xs s
-      else
-      match H u (get_input_vars md ft) md ft (flatten_term (head x)) s with
-      | Some sigma1 =>
-      let
-      '(fv, rs) := select u m ft md xs s in
-      (vars_sigma sigma1 `|` varsU_rule x `|` fv, (sigma1, premises x) :: rs)
-      | None => select u m ft md xs s
-      end).
-  Proof. by []. Qed. *)
-
-  Lemma select_consF sP ft x xs s:
+(*   Lemma select_consF sP ft x xs s:
     (* inl m = get_tm_hd (head x) -> *)
     select u sP ft (x::xs) s = 
     match H u sP (get_input_vars sP ft).1 ft (head x) s with
@@ -272,7 +299,7 @@ Section map.
       (vars_sigma sigma1 `|` varsU_rule x `|` fv, ((sigma1, premises x) :: rs))
     | None => select u sP ft xs s
     end.
-  Proof. by rewrite//=. Qed.
+  Proof. by rewrite//=. Qed. *)
 
   Lemma inl_map_get_tm_hdmap:
     inl map == get_tm_hd map.
@@ -286,7 +313,7 @@ Section map.
 
   Lemma fresh_tm_app s m f a: fresh_tm s m (app f a) = 
     ((fresh_tm (fresh_tm s m f).1 (fresh_tm s m f).2 a)).
-  Proof. by rewrite/=!push -surjective_pairing. Qed.
+  Proof. by rewrite/=!push. Qed.
 
   Lemma fresh_tm_P s r p: fresh_tm s r (Tm_P p) = (s, r). by []. Qed.
   (* Lemma getfmap12d: (get_input_vars [:: input;  input;  output] (flatten_term map12d)) = fset0.
@@ -301,8 +328,8 @@ Section map.
     by rewrite !eqxx/= !fsetU0.
   Qed.
 
-  Lemma rename_app fv f a v:
-    (rename fv (Tm_App f a) v).2 = 
+(*   Lemma rename_app fv f a v:
+    (rename fv v (Tm_App f a)).2 = 
     app
       (ren
       (fresh_tm (fresh_tm (vars f `|` vars a `|` fv) v f).1
@@ -310,66 +337,358 @@ Section map.
       (ren
       (fresh_tm (fresh_tm (vars f `|` vars a `|` fv) v f).1
       (fresh_tm (vars f `|` vars a `|` fv) v f).2 a).2 a).
-  Proof. by rewrite/rename/= !push/=. Qed.
+  Proof. by rewrite/rename/= !push/=. Qed. *)
+  
+  Lemma sum_pop x (S: {fset V}): IV x \notin S ->
+    (\max_(i <- (IV x |` S : {fset V})) (let 'IV n := i in n)) = (maxn x 
+      (\max_(i <- S) (let 'IV n := i in n)))%nat.
+  Proof.
+    rewrite (big_fsetD1 (IV x))/=; last by rewrite !inE eqxx.
+    move=> IV; rewrite !fsetDUl !rem1 eqxx !simpl_set.
+    by do 3 f_equal; apply/fsetDidPl; rewrite fdisjointX1.
+  Qed.
 
-  Goal exists f s, runT u p' fset0 fmap0 (TA (call map12d)) (One s) false f /\ deref s X = list24.
+  Lemma sum_pop0 x:
+    (\max_(i <- [fset IV x]) (let 'IV n := i in n)) = x.
+  Proof.
+    rewrite (big_fsetD1 (IV x))/=; last by rewrite !inE eqxx.
+    by rewrite rem1 eqxx/= big_nil maxn0.
+  Qed.
+
+  Local Lemma v_progP: fresh (v_prog (rules p')) = 13.
+  Proof.
+    by rewrite /v_prog/=/varsU_rule/varsU_rhead/varsU_rprem/= !simpl_set/maxn/=.
+  Qed.
+  
+   Check fresh_atoms.
+  
+  Lemma fresh_atoms_cons n m x xs:
+    fresh_atoms n m (x :: xs) =
+      let Fxs := fresh_atoms n m xs in
+      let Fx := fresh_atom Fxs.1.1 Fxs.1.2 x in
+      (Fx.1.1,Fx.1.2,(Fx.2::Fxs.2)).
+  Proof. by rewrite/= !push//=. Qed.
+
+  Local Lemma simpl_p (n:nat):
+    fresh_rules n (rules p') = (addn 6 n,
+       [:: {| head := app (app (app map (IV (5+n))) nil) nil; premises := [::] |};
+           {|
+             head :=
+               app (app (app map (IV n)) (app (app cons (IV n.+1)) (IV (2 + n))))
+                 (app (app cons (IV (3+n))) (IV (4+n)));
+             premises :=
+               [:: call (app (app (IV n) (IV n.+1)) (IV (3+n)));
+                   call (app (app (app map (IV n)) (IV (2+n))) (IV (4+n)))]
+           |};
+           {| head := app (app double one) two; premises := [::] |}]).
+  Proof.
+    rewrite/p' fresh_rules_cons.
+    set X := fresh_rules _ _.
+    rewrite /=FmapE.fmapE eqxx/=.
+    have: X = (addn 5 n,
+       [:: {|
+             head :=
+               app (app (app map (IV n)) (app (app cons (IV n.+1)) (IV (2+n))))
+                 (app (app cons (IV (3+n))) (IV (4+n)));
+             premises :=
+               [:: call (app (app (IV n) (IV n.+1)) (IV (3+n)));
+                   call (app (app (app map (IV n)) (IV (2+n))) (IV (4+n)))]
+           |};
+           {| head := app (app double one) two; premises := [::] |}]).
+      rewrite{}/X fresh_rules_cons.
+      set X := fresh_rules _ _.
+      have: X = (n,[:: {| head := app (app double one) two; premises := [::] |}]) by [].
+      move=> ->{X}.
+      set RF := fresh_rule _ _.
+      have: RF = (addn 5 n,
+           {|
+             head :=
+               app (app (app map (IV n)) (app (app cons (IV n.+1)) (IV (2+n))))
+                 (app (app cons (IV (3+n))) (IV (4+n)));
+             premises :=
+               [:: call (app (app (IV n) (IV n.+1)) (IV (3+n)));
+                   call (app (app (app map (IV n)) (IV (2+n))) (IV (4+n)))]
+           |}).
+        rewrite{}/RF/fresh_rule [premises _]/=[head _]/=.
+        rewrite [rename _ _ _]/=/rename [fresh_tm _ _ _]/=.
+        rewrite !inE orbF.
+        case: eqP => // _.
+        rewrite !inE.
+        do 2 case: eqP => // _.
+        rewrite orbF !inE.
+        do 3 case: eqP => // _.
+        sif.
+        rewrite !inE.
+        do 4 case: eqP => // _.
+        sif.
+        rewrite fresh_atoms_cons.
+        set FR := fresh_atoms _ _ _.
+        have: FR = (addn 5 n, [fmap].[F <- IV n].[X <- IV n.+1].[Y <- IV (2+n)].[X' <- IV (3+n)].[Y' <- IV (4+n)], [:: call (app (app (app map (IV n)) (IV (2+n))) (IV (4+n)))]).
+(*         have: FR = (addn 5 n, [fmap].[F <- IV n].[X <- IV n.+1].[Y <- IV (2+n))].[X' <- IV 16].[Y' <- IV 17], [:: call (app (app (app map (IV n)) (IV (2+n))) (IV 17))]). *)
+          rewrite{}/FR fresh_atoms_cons.
+          set FR := fresh_atoms _ _ _.
+          have: FR = (addn 5 n, [fmap].[F <- IV n].[X <- IV n.+1].[Y <- IV (2+n)].[X' <- IV (3+n)].[Y' <- IV (4+n)], [::]).
+            by [].
+          move=> ->{FR}; cbn zeta.
+          set FR := fresh_atom _ _ _.
+          have: FR = (addn 5 n, [fmap].[F <- IV n].[X <- IV n.+1].[Y <- IV (2+n)].[X' <- IV (3+n)].[Y' <- IV (4+n)], call (app (app (app map (IV n)) (IV (2+n))) (IV (4+n)))).
+            rewrite{}/FR/fresh_atom/rename.
+            set FR := fresh_tm _ _ _.
+            have: FR = (addn 5 n, [fmap].[F <- IV n].[X <- IV n.+1].[Y <- IV (2+n)].[X' <- IV (3+n)].[Y' <- IV (4+n)]).
+              rewrite{}/FR/= !inE eqxx orbT.
+              by rewrite !inE eqxx orbT !inE eqxx/=.
+            move=>->; rewrite !ren_app !ren_V !FmapE.fmapE.
+            by rewrite !eqxx/=.
+          by move=> /=->.
+        move=>->{FR}; cbn zeta.
+        set FR := fresh_atom _ _ _.
+        have: FR = (addn 5 n, [fmap].[F <- IV n].[X <- IV n.+1].[Y <- IV (2+n)].[X' <- 
+   IV (3+n)].[Y' <- IV (4+n)], call (app (app (IV n) (IV n.+1)) (IV (3+n)))).
+          rewrite{}/FR /fresh_atom/rename.
+          set FR := fresh_tm _ _ _.
+          have: FR = (addn 5 n, [fmap].[F <- IV n].[X <- IV n.+1].[Y <- IV (2+n)].[X' <- IV (3+n)].[Y' <- IV (4+n)]).
+            by rewrite{}/FR/= !inE eqxx orbT !inE orbT !inE orbT.
+          by move=> ->{FR}; rewrite !ren_app !ren_V !FmapE.fmapE eqxx/=.
+        move=> ->{FR}.
+        by rewrite/ren !FmapE.fmapE eqxx/=.
+      by move=> ->{RF}//.
+    move=> ->{X}//.
+  Qed.
+  
+  Check matching.
+  
+  Lemma matching_Vd f (v: V) t s: v \notin vars_sigma s -> v \notin f -> 
+    v \notin (vars t) -> matching f (Tm_V v) t s = Some s.[v <- deref s t].
+  Proof.
+    move=> /[dup]; rewrite {1}inE => /norP[vd vc] vs vf vt.
+    rewrite/matching/montanari_deref/montanari_pair.
+    rewrite not_in_deref/=; last rewrite fdisjointX1//.
+    rewrite montanari_equation (negbTE vf).
+    rewrite ifF; last first.
+      case: eqP => //; subst.
+      move: vc vt.
+      destruct t; rewrite//=!inE; case: eqP => //=vv1.
+      case: fndP => //= v1s + _.
+        by move=> +/= H; move=> /codom_varsP[]; exists v1,v1s; rewrite -H/= inE.
+      by move=> +[?]; subst.
+    rewrite ifF; last first.
+      move: (conj vt vc) => /norP.
+      apply: contraNF.
+      by move=> /fsubsetP-/(_ _ (vars_tm_deref_sub _ _)); rewrite inE orbC.
+    rewrite montanari_equation/=/deref_sigma; do 2 f_equal.
+    apply/fmapP => k.
+    case: fndP => ks; last by rewrite not_fnd.
+    rewrite ffunE valPE/derefkv in_fnd not_in_deref//= fsetU0 fdisjoint1X.
+    by apply/contra/vc => H; apply/codom_varsP; eexists _,ks.
+  Qed.
+  
+  Goal exists f s, runT u p' 0 fmap0 (Unexplored (call map12d)) (One s) false f /\ deref s X = list24.
   Proof.
     do 2 eexists.
+    rewrite/u.
     split.
       apply: StepT'=> //=; cycle 1.
+      { rewrite/bc ifF ?acyclic_sigma0//.
+      rewrite !simpl_set !maxnn /maxn simpl_p; sif.
+      set FR := select _ _ _ _ _.
+      have : FR = [:: ([fmap].[IV 13 <- Tm_P double].[IV 14 <- one].[IV 15 <- nil].[X <- 
+       app (app cons (IV 16)) (IV 17)],
+       [:: call (app (app (IV 13) (IV 14)) (IV 16));
+           call (app (app (app map (IV 13)) (IV 15)) (IV 17))])].
+        { rewrite{}/FR select_cons [head _]/=[premises _]/= get_input_vars_map12d.
+        rewrite/addn ![Nat.add _ _]/=.
+        rewrite/map12d/list12.
+        rewrite/H eqxx !FmapE.fmapE eqxx /mapS.
+        rewrite[omap _ _]/=; cbn match.
+        rewrite eqxx [lang.matching _]/= matching_Vd//?vars_sigma0//.
+        rewrite [omap _ _]/=; cbn match.
+        rewrite eqxx.
+        set W := matching _ _ _ _.
+        have : W = None.
+          by rewrite/W/matching/montanari_deref/montanari_pair/= montanari_equation.
+        move=> ->{W}; rewrite [omap _ _]/=.
+        cbn match; rewrite select_cons.
+        set X:= select _ _ _ _ _.
+        have: X = [::] by [].
+        move=> ->{X}; rewrite[head _]/=.
+        set X := get_input_vars _ _.
+        have: X.1 = fset0.
+          by rewrite/X/get_input_vars !FmapE.fmapE/= !simpl_set.
+        move=> ->{X}.
+        rewrite/H/= !FmapE.fmapE/=.
+        rewrite matching_Vd?vars_sigma0//=.
+        rewrite /matching/montanari_deref/montanari_pair/= montanari_equation/=.
+        rewrite !FmapE.fmapE/=.
+        rewrite !not_fnd//=.
+        rewrite /matching/montanari_deref/montanari_pair/= montanari_equation/=.
+        rewrite /matching/montanari_deref/montanari_pair/= montanari_equation/=.
+        rewrite /matching/montanari_deref/montanari_pair/= montanari_equation/=.
+        rewrite deref_sigma_not_in; last by rewrite/= !codom_vars_set !inE empty_rem codom_vars0 inE.
+        rewrite/derefkv/map_prod !deref_V !FmapE.fmapE/= not_fnd//=.
+        rewrite montanari_equation/=montanari_equation/=.
+        rewrite deref_sigma_not_in; last first.
+          rewrite codom_vars_set remf1_set empty_rem/= codom_vars_set empty_rem codom_vars0 !inE//.
+        (rewrite unify_Vr//; try by rewrite !inE); last first.
+          do 2 rewrite codom_vars_set !remf1_set empty_rem/=.
+          by rewrite codom_vars_set empty_rem codom_vars0 !fsetU0.
+        rewrite !deref_App !deref_V !FmapE.fmapE/= !not_fnd//=.
+      }
+      move=> ->{FR}.
+      rewrite/max_sigmas/=/vars_atoms/=/vars_sigma codom_vars_set !remf1_set empty_rem/=.
+      do 3 rewrite codom_vars_set ?remf1_set empty_rem/=.
+      by rewrite codom_vars0 !simpl_set/maxn/=.
+      }
+      apply: StepT => //=.
+      {
       rewrite/bc ifF ?acyclic_sigma0//.
-      rewrite !simpl_set.
-      rewrite !fresh_rules_cons !fstS !sndS.
-      rewrite !simpl_set.
-      set F0 := (_ `|` _).
-      set F1 := (_ `|` _).
-      set F2 := (_ `|` _).
-      rewrite select_consF// [head _]/=.
-      rewrite get_input_vars_map12d fmapIn?inE//.
-      case H: H => //.
-        exfalso; move: H; rewrite/map12d/H eqxx !FmapE.fmapE.
-        rewrite eqxx [omap _ _]/= /mapS [omap _ _]/=.
-        case M: matching => //.
-        rewrite [omap _ _]/=.
-        cbn match.
-        rewrite eqxx [omap _ _]/=.
-        rewrite/matching/montanari_deref/montanari_pair.
-        rewrite !ground_deref//; last first.
-          by rewrite/list12/ground/= !simpl_set.
-        by rewrite montanari_equation/=.
-      rewrite {H} select_consF.
-      rewrite head_fresh_rule [head _]/=.
-      rewrite get_input_vars_map12d/map12d premises_fresh_rule [head _]/=.
-      rewrite [vars _]/= !simpl_set [premises _]/=.
-      set F3 := (_ `|` _).
-      rewrite !rename_app !ren_app !ren_P.
-      rewrite [vars _]/= !simpl_set [vars _]/= !simpl_set.
-      set FT := (fresh_tm _ _ _).2.
-      rewrite/H eqxx !FmapE.fmapE eqxx [omap _ _]/= /mapS eqxx.
-      rewrite/u [lang.matching _]/=.
-      rewrite/matching/montanari_deref/montanari_pair.
-      rewrite !deref_empty montanari_equation [omap _ _]/=.
-      rewrite montanari_equation [omap _ _]/=.
-      cbn match; rewrite eqxx.
-      rewrite in_fnd.
-        apply/fsubsetP.
-          apply: fresh_tm_domf_sub.
-        apply/fsubsetP.
-          apply: fresh_tm_sub1.
-        by rewrite/= !inE eqxx.
-      move=> iFT; rewrite !deref_App !odflt_Some !deref_P.
-      rewrite deref_sigma0 not_in_deref; last first.
-        rewrite/= fsetU0 fdisjointX1 inE.
-        admit.
-      rewrite not_in_deref; last first.
-        admit.
-      rewrite 3!montanari_equation.
-      case: eqP => [H|_].
-        by exfalso; move: H; rewrite/ren; case: fndP => //.
-      case: eqP => [H|_].
-        by exfalso; move: H; rewrite/ren; case: fndP => //.
-      rewrite montanari_equation eqxx montanari_equation.
-      case: eqP => [H|_].
-        by exfalso; move: H; rewrite/ren; case: fndP => //.
-  Abort.
+      set X := fresh _.
+      have: X = 20.
+        rewrite{}/X deref_App !deref_V !FmapE.fmapE not_fnd//.
+        rewrite !simpl_set/=.
+        rewrite in_fnd?inE//.
+        move=> X; rewrite ffunE/={X}.
+        rewrite !FmapE.fmapE/=.
+        repeat rewrite codom_vars_set ?remf1_set empty_rem/=.
+        rewrite codom_vars0 !simpl_set.
+        by rewrite/maxn/=/addn![Nat.add _ _]/=.
+      move=> ->{X}.
+      rewrite simpl_p.
+      rewrite/addn ![Nat.add _ _]/=.
+      set FR := select _ _ _ _ _.
+      have : FR =  [:: ([fmap].[IV 16 <- Tm_P two].[IV 13 <- double].[IV 14 <- one].[
+        IV 15 <- nil].[X <- app (app cons two) (IV 17)], [::])].
+        { rewrite{}/FR select_cons [head _]/=[premises _]/=.
+          set FR := deref _ _.
+          have: FR = app (app double one) (IV 16).
+            by rewrite/FR !deref_App !deref_V !FmapE.fmapE/= not_fnd//=.
+          move=> ->{FR}.
+          set FR := get_input_vars _ _.
+          have: FR = (fset0, Some func).
+            by rewrite/FR/get_input_vars !FmapE.fmapE/= !simpl_set.
+          move=> ->{FR}.
+          rewrite/H select_cons [head _]/=[premises _]/=.
+          set FR := (get_input_vars _ _).1.
+          have: FR = fset0.
+            by rewrite/FR/get_input_vars !FmapE.fmapE/= !simpl_set.
+          move=> ->{FR}.
+          rewrite/H.
+          rewrite select_cons [select _ _ _ _ _]/= [head _]/=.
+          set FR := (get_input_vars _ _).1.
+          have: FR = fset0.
+            by rewrite/FR/get_input_vars !FmapE.fmapE/= !simpl_set.
+          move=> ->{FR}.
+          rewrite/H eqxx !FmapE.fmapE eqxx [omap _ _]/=/doubleS eqxx.
+          rewrite [lang.matching _]/= matching_refl [omap _ _]/=/=.
+          rewrite /unify/montanari_deref/montanari_pair.
+          rewrite deref_P deref_V not_fnd//?inE//.
+          rewrite !montanari_equation/=.
+          rewrite !montanari_equation/=.
+          rewrite !deref_sigma_set; only 2-5: by [].
+          rewrite /=/derefkv !deref_App.
+          rewrite !deref_P !deref_V !FmapE.fmapE/=.
+          by rewrite !not_fnd ?deref_sigma0//=.
+        }
+      move=> ->{FR}.
+      rewrite/max_sigmas/=/vars_sigma/vars_atoms/=.
+      repeat rewrite codom_vars_set ?remf1_set empty_rem/=.
+      rewrite codom_vars0 !simpl_set.
+      by rewrite/maxn/=.
+    apply/negbF.
+    rewrite !acyclic_sigma_set !inE !remf1_set empty_rem/=.
+    repeat rewrite codom_vars_set ?remf1_set empty_rem/=.
+    rewrite codom_vars0 !fsetU0 inE.
+    rewrite !fdisjointXU fdisjointX0 !fdisjointX1 !inE/= andbT.
+    rewrite !acyclic_sigma_set !inE !remf1_set empty_rem/=.
+    repeat rewrite codom_vars_set ?remf1_set empty_rem/=.
+    rewrite codom_vars0 !fsetU0 inE fdisjointX0 !andbT.
+    rewrite !acyclic_sigma_set !inE !remf1_set empty_rem/=.
+    repeat rewrite codom_vars_set ?remf1_set empty_rem/=.
+    rewrite codom_vars0 !fsetU0 inE fdisjointX0 !andbT.
+    by rewrite !acyclic_sigma_set !inE empty_rem acyclic_sigma0 codom_vars0/= fdisjointX0.
+    }
+    apply: StepT => //=.
+    {
+      rewrite/bc ifF ?acyclic_sigma0//.
+      rewrite/next_subst[next _ _]/=.
+      set X := fresh _.
+      have: X = 27.
+        rewrite{}/X deref_App !deref_V !FmapE.fmapE not_fnd//.
+        rewrite !simpl_set/=.
+        rewrite in_fnd?inE//.
+        move=> X; rewrite ffunE/={X}.
+        rewrite !FmapE.fmapE/=.
+        repeat rewrite codom_vars_set ?remf1_set empty_rem/=.
+        by rewrite codom_vars0 !simpl_set.
+      move=> ->{X}.
+      set FR:= deref _ _.
+      have: FR = app (app (app map double) nil) (IV 17).
+        rewrite/FR !deref_App !deref_V !FmapE.fmapE/= not_fnd//=.
+      move=> ->{FR}.
+      rewrite simpl_p.
+      set FR := select _ _ _ _ _.
+      have : FR = [:: ([fmap].[IV 17 <- Tm_P nil].[IV 16 <- two].[IV 13 <- double].[
+         IV 14 <- one].[IV 15 <- nil].[X <- app (app cons two) nil].[
+         IV 32 <- double], [::])].
+        { rewrite{}/FR select_cons [head _]/=[premises _]/=.
+        set FR := (get_input_vars _ _).1.
+        have: FR = fset0.
+          by rewrite/FR/get_input_vars !FmapE.fmapE/= !simpl_set.
+        move=> ->{FR}.
+        rewrite/addn ![Nat.add _ _]/=.
+        set FR := H _ _ _ _ _ _.
+        have: FR = Some
+          (func,
+           [fmap].[IV 17 <- Tm_P nil].[IV 16 <- two].[IV 13 <- double].[
+           IV 14 <- one].[IV 15 <- nil].[X <- app (app cons two) nil].[
+           IV 32 <- double]).
+          rewrite{}/FR/H/= !FmapE.fmapE/= matching_Vd//; last first.
+            rewrite/vars_sigma/=.
+            repeat rewrite codom_vars_set ?remf1_set empty_rem/=.
+            by rewrite codom_vars0 !simpl_set !inE.
+          rewrite/=matching_refl/=.
+          rewrite/unify/montanari_deref deref_P deref_V !FmapE.fmapE/=not_fnd//=.
+          rewrite /montanari_pair/= montanari_equation/=!montanari_equation/=.
+          rewrite !deref_sigma_set; only 2-7: by [].
+          rewrite deref_sigma0/derefkv !deref_App !deref_P !deref_V.
+          by rewrite !FmapE.fmapE/=.
+        move=> ->{FR}.
+        rewrite select_cons [head _]/=[premises _]/=.
+        set FR := H _ _ _ _ _ _.
+        have: FR = None.
+          rewrite{}/FR/H/=!FmapE.fmapE/= !simpl_set matching_Vd//; last first.
+            rewrite/vars_sigma/=.
+            repeat rewrite codom_vars_set ?remf1_set empty_rem/=.
+            by rewrite codom_vars0 !simpl_set !inE.
+          rewrite/=.
+          rewrite/matching/montanari_deref !deref_App !deref_P !deref_V !FmapE.fmapE/=!not_fnd//=.
+          by rewrite /montanari_pair montanari_equation/=.
+        by move=> ->/=.
+        }
+      move=> ->{FR}//.
+      apply:negbF.
+      rewrite /next_subst[next _ _]/=.
+      rewrite !acyclic_sigma_set !inE !remf1_set empty_rem/=.
+      repeat rewrite codom_vars_set ?remf1_set empty_rem/=.
+      rewrite codom_vars0 !fsetU0 inE fdisjointXU fdisjointX0 !fdisjointX1 !inE/= !andbT.
+      
+      rewrite !acyclic_sigma_set !inE !remf1_set empty_rem/=.
+      repeat rewrite codom_vars_set ?remf1_set empty_rem/=.
+      rewrite codom_vars0 !fsetU0 inE fdisjointX0 !andbT.
+      
+      rewrite !acyclic_sigma_set !inE !remf1_set empty_rem/=.
+      repeat rewrite codom_vars_set ?remf1_set empty_rem/=.
+      rewrite codom_vars0 !fsetU0 inE fdisjointX0 !andbT.
+      
+      rewrite !acyclic_sigma_set !inE !remf1_set empty_rem/=.
+      repeat rewrite codom_vars_set ?remf1_set empty_rem/=.
+      rewrite codom_vars0 !fsetU0 inE fdisjointX0 !andbT.
+      
+      by rewrite !acyclic_sigma_set !inE empty_rem acyclic_sigma0 codom_vars0 fdisjointX0 inE.
+      
+      }
+      apply: StopOT => //=.
+      by [].
+    rewrite/next_subst[next _ _]/=/X.
+    by rewrite deref_V !FmapE.fmapE/=.
+  Qed.
 End map.
